theories/CTree/Logic/Trans.v
@@ -33,7 +33,8 @@ Notation ctreeEW E := (ctree (writerE (Bar E))).
 
 Section CTreeTrans.
   Context {E: Type} `{HE: Encode E} {X: Type}.
-
+  Notation encode := (@encode E HE).
+  
   (* Note: This Kripke transition rel observes labels, this is important
      for the [ktrans_bind_inv] lemma *)
   Variant ktrans_: relation (ctree E X * World E) :=    
@@ -120,6 +121,7 @@ Global Hint Constructors ktrans_: core.
 
 Section CTreeTrans.
   Context {E: Type} `{HE: Encode E}.
+  Notation encode := (@encode E HE).
   Local Open Scope ctl_scope.
   Notation sbisim := (fun (X: Type) => @sbisim E E HE HE X X eq).
 
@@ -142,7 +144,7 @@ Section CTreeTrans.
   Defined.
   Next Obligation.
     intros (t' & w' & TR).
-    ktrans_inv TR; contradiction.
+    ktrans_inv TR; apply H; constructor. 
   Defined.
 
   (*| Lemmas that depend on structure of [ctrees] |*)
@@ -151,8 +153,8 @@ Section CTreeTrans.
         (exists (i: fin' n), (k i, w) ↦ (t', w')).
   Proof.
     split; intro H.
-    - ktrans_inv H; apply trans_brD_inv in H as (n' & ?); exists n';
-        apply ktrans_trans; eexists.
+    - ktrans_inv H; apply trans_brD_inv in H as (n' & ?);
+        exists n'; apply ktrans_trans; eexists.
       + split; [eassumption|split]; auto. 
       + split; [eassumption|split]; auto.
         right; left; eauto.
@@ -189,7 +191,7 @@ Section CTreeTrans.
   Qed.
   
   Lemma ktrans_guard {X}: forall (t t': ctree E X) s s',
-      (guard t, s) ↦ (t', s') <-> (t, s) ↦ (t', s').
+      ktrans_ (guard t, s) (t', s') <-> ktrans_ (t, s) (t', s').
   Proof.
     intros; split; intros.
     - now apply ktrans_brD in H as (i & ?). 
@@ -197,7 +199,7 @@ Section CTreeTrans.
   Qed.
 
   Lemma ktrans_ret {X}: forall (t: ctree E X) s s' x,
-      (Ret x, s) ↦ (t, s') <-> (s' = Done x /\ t ≅ stuck /\ ~ is_done s).
+      ktrans_ (Ret x, s) (t, s') <-> (s' = Done x /\ t ≅ stuck /\ ~ is_done s).
   Proof.
     intros; split; intros.
     - ktrans_inv H; dependent destruction H; auto.
@@ -205,7 +207,7 @@ Section CTreeTrans.
       apply KtransRet; etrans.
   Qed.
 
-  Lemma ktrans_vis {X}: forall (t: ctree E X) (s s': World E) (e: E) (k: encode e -> ctree E X),
+  Lemma ktrans_vis{X}: forall (t: ctree E X) (s s': World E) (e: E) (k: encode e -> ctree E X),
       ktrans_ (Vis e k, s) (t, s') <->
       (exists (x: encode e), s' = Obs e x /\ k x ≅ t /\ ~ is_done s).
   Proof.
@@ -224,7 +226,23 @@ Section CTreeTrans.
       right; left; eauto.
   Qed.
 
-  Lemma ktrans_bind_l: forall {X Y} w w' (t t': ctree E Y) (k: Y -> ctree E X),
+  Lemma ktrans_not_started{X}: forall (t t': ctree E X) w,
+      ktrans_ (t, w) (t', NotStarted) ->
+        w = NotStarted.
+  Proof.
+    intros * H.
+    inv H; reflexivity.
+  Qed.
+
+  Lemma ktrans_not_done{X}: forall (t t': ctree E X) w w',
+    (t, w) ↦ (t', w') ->
+    ~ is_done w.
+  Proof.
+    intros; inv H; auto.
+  Qed.
+  Hint Resolve ktrans_not_done: ctl.
+            
+  Lemma ktrans_bind_l{X Y}: forall (t t': ctree E Y) (k: Y -> ctree E X) w w',
       ktrans_ (t, w) (t', w') ->
       ~ is_done w' ->
       ktrans_ (x <- t ;; k x, w) (x <- t' ;; k x, w').
@@ -234,91 +252,79 @@ Section CTreeTrans.
     - exists tau; split. (* BrS *)
       + apply trans_bind_l; auto.
         intro Hcontra; inv Hcontra.
-      + split; auto.
+      + split; auto with ctl.
     - exists (obs e x); split. (* Vis *)
       + apply trans_bind_l; auto.
-        intro Hcontra; inv Hcontra.
-      + split; try assumption.
+        intro Hcontra; inv Hcontra; world_inv.
+      + split; auto with ctl. (* Ret *)
         right; eauto.
-    - exfalso.
-      apply H0; econstructor.
+    - exfalso; apply H0; constructor. 
   Qed.
 
-  Lemma ktrans_bind_r{X Y}: forall w w' (t: ctree E Y) (u: ctree E X)
-                              (k: Y -> ctree E X) (x: Y),
-      ktrans_ (t, w) (stuck, Done x) ->
-      ktrans_ (k x, w) (u, w') ->
-      ktrans_ (x <- t ;; k x, w) (u, w').
+  Lemma ktrans_bind_r{X Y}: forall (t: ctree E Y) (u: ctree E X) (k: Y -> ctree E X) (y: Y) w w',
+      ktrans_ (t, w) (stuck, Done y) ->
+      ktrans_ (k y, w) (u, w') ->
+      ktrans_ (y <- t ;; k y, w) (u, w').
   Proof.
     intros.
-    ktrans_inv H.
-    - exfalso; apply H1; econstructor.
-    - inv Heqw.
-    - inv Heqw; invert.
-      ktrans_inv H0; apply ktrans_trans.
+    ktrans_inv H; apply ktrans_trans.
+    - exfalso; apply H1; constructor.
+    - world_inv.
+    - ktrans_inv H0; world_inv.
       + exists tau; split.
-        * apply trans_bind_r with x0; etrans. 
+        * apply trans_bind_r with x; etrans. 
         * split; auto.
-      + exists (obs e x); split.
-        * apply trans_bind_r with x0; etrans.
-        * split; [auto|].
+      + exists (obs e x0); split.
+        * apply trans_bind_r with x; etrans.
+        * split; auto.
           right; left; eauto.
-      + exists (val x); split.
-        * apply trans_bind_r with x0; etrans.
-        * split; [auto|].
+      + exists (val x0); split.
+        * apply trans_bind_r with x; etrans.
+        * split; auto.
           right; right; eauto.
   Qed.
-  
-  Lemma ktrans_bind_inv{X Y}:
-    forall w w' (t: ctree E Y) (u: ctree E X) (k: Y -> ctree E X),
+
+  Lemma ktrans_bind_inv{X Y}: forall (t: ctree E Y) (u: ctree E X) (k: Y -> ctree E X) w w',
       ktrans_ (x <- t ;; k x, w) (u, w') ->
-      ( ~ is_done w' /\ exists t', ktrans_ (t, w) (t', w') /\ u ≅ x <- t' ;; k x) \/
-        ( exists x, ktrans_ (t, w) (stuck, Done x) /\ ktrans_ (k x, w) (u, w')).
+      (exists t', ktrans_ (t, w) (t', w')
+             /\ u ≅ x <- t' ;; k x) \/
+      (exists y, ktrans_ (t, w) (stuck, Done y)
+            /\ ktrans_ (k y, w) (u, w')).
   Proof.
     intros * TR.
     ktrans_inv TR; destruct (trans_bind_inv _ _ TR) as
-      [(Hv & t' & TR' & Heq) | (x' & TRv & TR')].
-    + left; split; auto.
-      exists t'; split; cbn; auto.
-    + right; exists x'; split; cbn; auto.
-    + left; split; auto.
-      * intros Hcontra; inv Hcontra.
-      * exists t'; split; cbn; auto.
-    + right; exists x'; split; cbn; auto.
-    + exfalso; apply Hv; econstructor.
-    + right.
-      exists x'; split; apply ktrans_trans.
-      * exists (val x'); split; auto; split; auto.
-        right; right; eauto.
-      * exists (val x); split; auto; split; auto.
-        right; right; eauto.
+      [(Hv & t' & TR' & Heq) | (y & TRv & TR')]. 
+    + left; exists t'; split; auto.
+    + right; exists y; split; apply ktrans_trans.
+      * exists (val y); split; auto; split; auto with ctl.
+        right; right; exists y; auto.
+      * exists (tau); split; auto.
+    + left; exists t'; split; auto with ctl.
+    + right; exists y; cbn; auto with ctl.
+    + exfalso; apply Hv; constructor.
+    + right; exists y; cbn; split; auto.
+      apply ktrans_trans.
+      exists (val x); split; [|split]; auto.
+      right; right; exists x; auto.
   Qed.
 
-  Lemma ktrans_bind_inv_l{X Y}: forall w w' (t: ctree E Y) (u: ctree E X)
-                                  (k: Y -> ctree E X),
-      ktrans_ (x <- t ;; k x, w) (u, w') ->      
-      (exists t' w'', ktrans_ (t, w) (t', w'')).
-  Proof.
-    intros.
-    apply ktrans_bind_inv in H.
-    destruct H as [(? & ? & ? & ?) | (x0 & Hret & Hcont)]; eauto.
-  Qed.
-
-  Local Typeclasses Transparent equ.
-  Lemma ktrans_trigger_inv {X}:
-    forall w w' (e: E) (k: encode e -> ctree E X) (u': ctree E X),
-      ktrans_ (x <- trigger e ;; k x, w) (u', w') ->
-      exists (x: encode e), u' ≅ k x /\ w' = Obs e x.
-  Proof.    
-    intros.
-    apply ktrans_bind_inv in H.
-    destruct H as [(? & ? & ? & ?) | (x0 & Hret & Hcont)].
-    - unfold trigger in H0.
-      apply ktrans_vis in H0 as (x' & ? & ? & ?).
-      unfold resum, ReSum_refl, resum_ret, ReSumRet_refl in *; subst.
-      exists x'; split; setoid_rewrite <- H2 in H1; rewrite bind_ret_l in H1; auto.
-    - dependent destruction Hret; exfalso; apply H0; auto with ctl.
-      unfold trans in H; dependent destruction H.
-  Qed.
- 
 End CTreeTrans.
+
+Local Typeclasses Transparent equ.
+Lemma ktrans_trigger_inv `{ReSumRet E1 E2} {X}: forall (e: E2) w w' (k: encode (resum e) -> ctree E2 X) (u': ctree E2 X),
+      ktrans_ (z <- trigger e ;; k z, w) (u', w') ->
+      (exists z, w' = Obs e z /\ u' ≅ k z).
+Proof.    
+  intros.
+  unfold trigger in H3.
+  destruct w'.
+  - rewrite bind_vis in H3.
+    apply ktrans_vis in H3 as (? & ? & ?); world_inv.
+  - apply ktrans_bind_inv in H3 as [(? & ? & ?) | (x0 & Hret & Hcont)].
+    + apply ktrans_vis in H3 as (y & ? & ? & ?).
+      unfold resum, ReSum_refl, resum_ret, ReSumRet_refl in *; world_inv.
+      exists y; setoid_rewrite <- H5 in H4; rewrite bind_ret_l in H4; auto.
+    + apply ktrans_vis in Hret as (? & ? & ?); world_inv. 
+  - rewrite bind_vis in H3.
+    apply ktrans_vis in H3 as (? & ? & ?); world_inv. 
+Qed.
